add basic if |= if example

theories/Automation.v
@@ -1,4 +1,5 @@
 
+From Coq Require Import ZArith.
 From ITree Require Export ITree.
 From Paco Require Import paco.
 Require Export Refinement.
@@ -39,4 +40,101 @@ Lemma padded_refines_if_r E1 E2 RE REAns R1 R2 RR (t1 : itree_spec E1 R1) (t2 t3
   padded_refines RE REAns RR t1 (if b then t2 else t3).
 Proof.
   intros. destruct b; eauto.
+Qed.
+
+
+(** * Hints *)
+
+Create HintDb refines.
+
+Hint Extern 999 (padded_refines _ _ _ _ _) => shelve : refines.
+
+(** ** IntroArg *)
+
+Inductive ArgName := Any | If.
+Ltac argName n :=
+  match n with
+  | Any      => fresh "a"
+  | If       => fresh "e_if"
+  end.
+
+Definition IntroArg (n : ArgName) A (goal : A -> Prop) := forall a, goal a.
+
+Hint Opaque IntroArg : refines.
+
+Lemma IntroArg_fold n A goal : forall a, IntroArg n A goal -> goal a.
+Proof. intros a H; exact (H a). Qed.
+
+(* Lemma IntroArg_unfold n A (goal : A -> Prop) : (forall a, goal a) -> IntroArg n A goal. *)
+(* Proof. unfold IntroArg; intro H; exact H. Qed. *)
+
+Ltac IntroArg_intro e := intro e.
+
+Ltac IntroArg_forget := let e := fresh in intro e; clear e.
+
+Ltac IntroArg_intro_dependent_destruction n :=
+  let e := argName n in
+    IntroArg_intro e; dependent destruction e.
+
+Ltac IntroArg_base_tac n A g :=
+  lazymatch A with
+  | true  = true  => IntroArg_intro_dependent_destruction n
+  | false = false => IntroArg_intro_dependent_destruction n
+  | true  = false => IntroArg_intro_dependent_destruction n
+  | false = true  => IntroArg_intro_dependent_destruction n
+  end.
+
+Hint Extern 1 (IntroArg ?n ?A ?g) => IntroArg_base_tac n A g : refines.
+
+Ltac IntroArg_rewrite_bool_eq n :=
+  let e := fresh in
+    IntroArg_intro e; repeat rewrite e in *;
+    apply (IntroArg_fold n _ _ e); clear e.
+
+Hint Extern 2 (IntroArg ?n (@eq bool _ _) _) =>
+  progress (IntroArg_rewrite_bool_eq n) : refines.
+
+Hint Extern 5 (IntroArg ?n (?x = ?y) _) =>
+  let e := argName n in IntroArg_intro e;
+    try first [ is_var x; subst x | is_var y; subst y ] : refines.
+Hint Extern 6 (IntroArg ?n _ _) =>
+  let e := argName n in IntroArg_intro e : refines.
+
+(** ** Main refinement rules *)
+
+Definition padded_refines_if_l_IntroArg E1 E2 RE REAns R1 R2 RR t1 t2 t3 b :
+  (IntroArg If (b = true) (fun _ => padded_refines RE REAns RR t1 t3)) ->
+  (IntroArg If (b = false) (fun _ => padded_refines RE REAns RR t2 t3)) ->
+  padded_refines RE REAns RR (if b then t1 else t2) t3 :=
+  padded_refines_if_l E1 E2 RE REAns R1 R2 RR t1 t2 t3 b.
+Definition padded_refines_if_r_IntroArg E1 E2 RE REAns R1 R2 RR t1 t2 t3 b :
+  (IntroArg If (b = true) (fun _ => padded_refines RE REAns RR t1 t2)) ->
+  (IntroArg If (b = false) (fun _ => padded_refines RE REAns RR t1 t3)) ->
+  padded_refines RE REAns RR t1 (if b then t2 else t3) :=
+  padded_refines_if_r E1 E2 RE REAns R1 R2 RR t1 t2 t3 b.
+
+Hint Extern 1 (padded_refines _ _ _ (if _ then _ else _) _) =>
+  apply padded_refines_if_l_IntroArg : refines.
+Hint Extern 1 (padded_refines _ _ _ _ (if _ then _ else _)) =>
+  apply padded_refines_if_r_IntroArg : refines.
+
+Hint Extern 3 (padded_refines _ _ _ (Ret _) (Ret _)) =>
+  apply padded_refines_ret; (reflexivity || shelve) : refines.
+
+
+(** * Tactics *)
+
+Ltac prove_refinement := unshelve (typeclasses eauto with refines).
+
+
+(** * Examples *)
+
+Open Scope Z_scope.
+
+Lemma test E x :
+  @padded_refines E E _ _ eqE eqEAns eq
+                  (if x >=? 0 then if x <? 256 then Ret 1 else Ret 0 else Ret 0)
+                  (if x <? 256 then if x >=? 0 then Ret 1 else Ret 0 else Ret 0).
+Proof.
+  prove_refinement.
 Qed.
